instruction selection: `constant`, `add` refinement proof (#416)
We prove the correctness of the lowering pattern for `constant` and
`add`. If we agree on this format and organization I will write more
proofs and push them. Note that the proof for `constant` does not deal
with `.poison`, as `llvm.constant` is never poison.

I think we have two options to consider wrt. lemmas' formulation: 
* wrapping the semantics of the `unrealized_conversion_cast`
(i.e.,`toReg : i64 -> !reg`) directly in the lemma and proving the
refinement `i64` to `!reg`.
* wrapping the semantics of the `unrealized_conversion_cast` *in both
directions* (i.e.,`toReg : i64 -> !reg` and `toInt : !reg -> i64`). This
would be more consistent with what the rewriter actually does, and the
refinement goes from `i64` to `i64`.

I am pushing both option and look forward to gathering opinions :)

Also, the tactic is the usual:
* unwrap semantics
* split + get rid of monad
* `bv_decide`

If we agree on these steps we can wrap it into an actual tactic, as we
did in `lean-MLIR` (for a subsequent PR).

Veir/Data/Refinement.lean
@@ -9,11 +9,16 @@ public section
   This file defines the refinement relation from the `LLVM.Int` to `RISCV.Reg` type.
 -/
 
-
 /--
-  `LLVM.Int` is refined by `RISCV.Reg`.
+  `LLVM.Int` is refined by `LLVM.Int`.
+  `i'` refines `i` if its behaviour are a subset of the behaviours allowed by `i`.
+  In particular, any concrete `i'` refines a poison `i`, but a poison `i'` does *not* refine
+  any `i`.
 -/
-def IntIsRefinedByReg [DecidableEq Prop] (i : Veir.Data.LLVM.Int 64) (r : Veir.Data.RISCV.Reg) : Prop :=
+def isRefinedBy (i i' : Veir.Data.LLVM.Int 64) : Prop :=
   match i with
-  | .val v => r.val = v
+  | .val v =>
+    match i' with
+    | .val v' => v = v'
+    | .poison => true
   | .poison => true
