Veir/Passes/InstructionSelection/Proofs.lean
@@ -1,6 +1,7 @@
 import Veir.Data.RISCV.Reg.Basic
 import Veir.Data.LLVM.Int.Basic
 import Veir.Data.Casting
+import Veir.Data.Refinement
 import Std.Tactic.BVDecide
 
 /-!
@@ -8,7 +9,7 @@ import Std.Tactic.BVDecide
   instruction selection rewrites.
 -/
 
-open Veir
+namespace Veir.Data.RISCV
 
 /--
   Prove the correctness of the `constant` lowering pattern.
@@ -16,6 +17,24 @@ open Veir
   We do not need to consider the poison case, as the semantics of `llvm_constant`
   are always concrete in the interpreter.
 -/
-theorem constant_val (v : BitVec 64) :
-    (Data.LLVM.Int.val v) = RISCV.Reg.toInt (Data.RISCV.li v) 64 := by
-  simp [Data.RISCV.li, RISCV.Reg.toInt]
+theorem constant_refinement:
+    isRefinedBy (LLVM.Int.constant 64 v) (RISCV.Reg.toInt (Data.RISCV.li (BitVec.ofInt 64 v)) 64) := by
+  simp [isRefinedBy, Data.LLVM.Int.constant, Data.RISCV.li, RISCV.Reg.toInt]
+
+/--
+  Prove the correctness of the `add` lowering pattern.
+-/
+theorem add_refinement:
+    isRefinedBy (Data.LLVM.Int.add x y) (RISCV.Reg.toInt (Data.RISCV.add (LLVM.Int.toReg x) (LLVM.Int.toReg y)) 64) := by
+  simp only [isRefinedBy, Data.LLVM.Int.add, Bool.false_eq_true, false_and, ↓reduceIte,
+    pure_bind, RISCV.Reg.toInt, Data.RISCV.add, LLVM.Int.toReg, BitVec.truncate_eq_setWidth,
+    BitVec.setWidth_eq]
+  split
+  · split
+    · split
+      <;> bv_decide
+    · split
+      · bv_decide
+      · simp only [Id.run, Data.LLVM.Int.val.injEq] at *
+        bv_decide
+  · bv_decide
